code/bignum/Hacl.Bignum.Exponentiation.fst
@@ -24,39 +24,39 @@ friend Hacl.Spec.Bignum.Exponentiation
 
 #reset-options "--z3rlimit 50 --fuel 0 --ifuel 0"
 
-let bn_mod_exp #t k bn_mod_exp_precompr2 nBits n a bBits b res =
+let bn_mod_exp_raw #t k bn_mod_exp_raw_precompr2 nBits n a bBits b res =
   [@inline_let] let len = k.BM.bn.BN.len in
   push_frame ();
   let r2 = create len (uint #t #SEC 0) in
   BM.precomp nBits n r2;
-  bn_mod_exp_precompr2 n a bBits b r2 res;
+  bn_mod_exp_raw_precompr2 n a bBits b r2 res;
   pop_frame ()
 
 
-let bn_mod_exp_mont_ladder #t k bn_mod_exp_mont_ladder_precompr2 nBits n a bBits b res =
+let bn_mod_exp_ct #t k bn_mod_exp_ct_precompr2 nBits n a bBits b res =
   [@inline_let] let len = k.BM.bn.BN.len in
   push_frame ();
   let r2 = create len (uint #t #SEC 0) in
   BM.precomp nBits n r2;
-  bn_mod_exp_mont_ladder_precompr2 n a bBits b r2 res;
+  bn_mod_exp_ct_precompr2 n a bBits b r2 res;
   pop_frame ()
 
 
-let bn_mod_exp_fw #t k bn_mod_exp_fw_precompr2 nBits n a bBits b l res =
+let bn_mod_exp_fw_raw #t k bn_mod_exp_fw_raw_precompr2 nBits n a bBits b l res =
   [@inline_let] let len = k.BM.bn.BN.len in
   push_frame ();
   let r2 = create len (uint #t #SEC 0) in
   BM.precomp nBits n r2;
-  bn_mod_exp_fw_precompr2 n a bBits b l r2 res;
+  bn_mod_exp_fw_raw_precompr2 n a bBits b l r2 res;
   pop_frame ()
 
 
-let bn_mod_exp_fw_ct #t k bn_mod_exp_fw_precompr2_ct nBits n a bBits b l res =
+let bn_mod_exp_fw_ct #t k bn_mod_exp_fw_ct_precompr2 nBits n a bBits b l res =
   [@inline_let] let len = k.BM.bn.BN.len in
   push_frame ();
   let r2 = create len (uint #t #SEC 0) in
   BM.precomp nBits n r2;
-  bn_mod_exp_fw_precompr2_ct n a bBits b l r2 res;
+  bn_mod_exp_fw_ct_precompr2 n a bBits b l r2 res;
   pop_frame ()
 
 
@@ -66,26 +66,26 @@ let bn_mod_exp_fw_ct #t k bn_mod_exp_fw_precompr2_ct nBits n a bBits b l res =
 let bn_check_mod_exp_u32 (len:BN.meta_len U32) : bn_check_mod_exp_st U32 len =
   bn_check_mod_exp (BM.mk_runtime_mont len)
 [@CInline]
-let bn_mod_exp_precompr2_u32 (len:BN.meta_len U32) : bn_mod_exp_precompr2_st U32 len =
-  bn_mod_exp_precompr2 (BM.mk_runtime_mont len)
+let bn_mod_exp_raw_precompr2_u32 (len:BN.meta_len U32) : bn_mod_exp_raw_precompr2_st U32 len =
+  bn_mod_exp_raw_precompr2 (BM.mk_runtime_mont len)
 [@CInline]
-let bn_mod_exp_mont_ladder_precompr2_u32 (len:BN.meta_len U32) : bn_mod_exp_mont_ladder_precompr2_st U32 len =
-  bn_mod_exp_mont_ladder_precompr2 (BM.mk_runtime_mont len)
+let bn_mod_exp_ct_precompr2_u32 (len:BN.meta_len U32) : bn_mod_exp_ct_precompr2_st U32 len =
+  bn_mod_exp_ct_precompr2 (BM.mk_runtime_mont len)
 [@CInline]
-let bn_mod_exp_fw_precompr2_u32 (len:BN.meta_len U32) : bn_mod_exp_fw_precompr2_st U32 len =
-  bn_mod_exp_fw_precompr2 (BM.mk_runtime_mont len)
+let bn_mod_exp_fw_raw_precompr2_u32 (len:BN.meta_len U32) : bn_mod_exp_fw_precompr2_st U32 len =
+  bn_mod_exp_fw_raw_precompr2 (BM.mk_runtime_mont len)
 [@CInline]
-let bn_mod_exp_fw_precompr2_ct_u32 (len:BN.meta_len U32) : bn_mod_exp_fw_precompr2_st U32 len =
-  bn_mod_exp_fw_precompr2_ct (BM.mk_runtime_mont len)
+let bn_mod_exp_fw_ct_precompr2_u32 (len:BN.meta_len U32) : bn_mod_exp_fw_precompr2_st U32 len =
+  bn_mod_exp_fw_ct_precompr2 (BM.mk_runtime_mont len)
 
 inline_for_extraction noextract
 let mk_runtime_exp_u32 (len:BN.meta_len U32) : exp U32 = {
   mont = BM.mk_runtime_mont len;
   exp_check = bn_check_mod_exp_u32 len;
-  mod_exp_precomp = bn_mod_exp_precompr2_u32 len;
-  ct_mod_exp_precomp = bn_mod_exp_mont_ladder_precompr2_u32 len;
-  mod_exp_fw_precomp = bn_mod_exp_fw_precompr2_u32 len;
-  ct_mod_exp_fw_precomp = bn_mod_exp_fw_precompr2_ct_u32 len;
+  raw_mod_exp_precomp = bn_mod_exp_raw_precompr2_u32 len;
+  ct_mod_exp_precomp = bn_mod_exp_ct_precompr2_u32 len;
+  raw_mod_exp_fw_precomp = bn_mod_exp_fw_raw_precompr2_u32 len;
+  ct_mod_exp_fw_precomp = bn_mod_exp_fw_ct_precompr2_u32 len;
   }
 
 
@@ -93,26 +93,26 @@ let mk_runtime_exp_u32 (len:BN.meta_len U32) : exp U32 = {
 let bn_check_mod_exp_u64 (len:BN.meta_len U64) : bn_check_mod_exp_st U64 len =
   bn_check_mod_exp (BM.mk_runtime_mont len)
 [@CInline]
-let bn_mod_exp_precompr2_u64 (len:BN.meta_len U64) : bn_mod_exp_precompr2_st U64 len =
-  bn_mod_exp_precompr2 (BM.mk_runtime_mont len)
+let bn_mod_exp_raw_precompr2_u64 (len:BN.meta_len U64) : bn_mod_exp_raw_precompr2_st U64 len =
+  bn_mod_exp_raw_precompr2 (BM.mk_runtime_mont len)
 [@CInline]
-let bn_mod_exp_mont_ladder_precompr2_u64 (len:BN.meta_len U64) : bn_mod_exp_mont_ladder_precompr2_st U64 len =
-  bn_mod_exp_mont_ladder_precompr2 (BM.mk_runtime_mont len)
+let bn_mod_exp_ct_precompr2_u64 (len:BN.meta_len U64) : bn_mod_exp_ct_precompr2_st U64 len =
+  bn_mod_exp_ct_precompr2 (BM.mk_runtime_mont len)
 [@CInline]
-let bn_mod_exp_fw_precompr2_u64 (len:BN.meta_len U64) : bn_mod_exp_fw_precompr2_st U64 len =
-  bn_mod_exp_fw_precompr2 (BM.mk_runtime_mont len)
+let bn_mod_exp_fw_raw_precompr2_u64 (len:BN.meta_len U64) : bn_mod_exp_fw_precompr2_st U64 len =
+  bn_mod_exp_fw_raw_precompr2 (BM.mk_runtime_mont len)
 [@CInline]
-let bn_mod_exp_fw_precompr2_ct_u64 (len:BN.meta_len U64) : bn_mod_exp_fw_precompr2_st U64 len =
-  bn_mod_exp_fw_precompr2_ct (BM.mk_runtime_mont len)
+let bn_mod_exp_fw_ct_precompr2_u64 (len:BN.meta_len U64) : bn_mod_exp_fw_precompr2_st U64 len =
+  bn_mod_exp_fw_ct_precompr2 (BM.mk_runtime_mont len)
 
 inline_for_extraction noextract
 let mk_runtime_exp_u64 (len:BN.meta_len U64) : exp U64 = {
   mont = BM.mk_runtime_mont len;
   exp_check = bn_check_mod_exp_u64 len;
-  mod_exp_precomp = bn_mod_exp_precompr2_u64 len;
-  ct_mod_exp_precomp = bn_mod_exp_mont_ladder_precompr2_u64 len;
-  mod_exp_fw_precomp = bn_mod_exp_fw_precompr2_u64 len;
-  ct_mod_exp_fw_precomp = bn_mod_exp_fw_precompr2_ct_u64 len;
+  raw_mod_exp_precomp = bn_mod_exp_raw_precompr2_u64 len;
+  ct_mod_exp_precomp = bn_mod_exp_ct_precompr2_u64 len;
+  raw_mod_exp_fw_precomp = bn_mod_exp_fw_raw_precompr2_u64 len;
+  ct_mod_exp_fw_precomp = bn_mod_exp_fw_ct_precompr2_u64 len;
   }
 
 
