code/bignum/Hacl.Bignum.SafeAPI.fst
@@ -178,40 +178,40 @@ let bn_mod_exp_safe_st (t:limb_t) (len:BN.meta_len t) =
 
 
 inline_for_extraction noextract
-val bn_mod_exp_safe: #t:limb_t -> k:BE.exp t -> bn_mod_exp_safe_st t k.BE.mont.BM.bn.BN.len
-let bn_mod_exp_safe #t k n a bBits b res =
+val bn_mod_exp_raw_safe: #t:limb_t -> k:BE.exp t -> bn_mod_exp_safe_st t k.BE.mont.BM.bn.BN.len
+let bn_mod_exp_raw_safe #t k n a bBits b res =
   [@inline_let] let len = k.BE.mont.BM.bn.BN.len in
   let h0 = ST.get () in
   let is_valid_m = k.BE.exp_check n a bBits b in
   let nBits = size (bits t) *! BB.unsafe_size_from_limb (BL.bn_get_top_index len n) in
 
-  BE.bn_mod_exp k.BE.mont k.BE.mod_exp_precomp nBits n a bBits b res;
+  BE.bn_mod_exp_raw k.BE.mont k.BE.raw_mod_exp_precomp nBits n a bBits b res;
   let h1 = ST.get () in
   mapT len res (logand is_valid_m) res;
   SD.bn_mask_lemma (as_seq h1 res) is_valid_m;
 
   if BB.unsafe_bool_of_limb is_valid_m then begin
     SL.bn_low_bound_bits_lemma #t #(v len) (as_seq h0 n);
-    SE.bn_mod_exp_lemma (v len) (v nBits) (as_seq h0 n) (as_seq h0 a) (v bBits) (as_seq h0 b) end;
+    SE.bn_mod_exp_raw_lemma (v len) (v nBits) (as_seq h0 n) (as_seq h0 a) (v bBits) (as_seq h0 b) end;
   BB.unsafe_bool_of_limb is_valid_m
 
 
 inline_for_extraction noextract
-val bn_mod_exp_mont_ladder_safe: #t:limb_t -> k:BE.exp t -> bn_mod_exp_safe_st t k.BE.mont.BM.bn.BN.len
-let bn_mod_exp_mont_ladder_safe #t k n a bBits b res =
+val bn_mod_exp_ct_safe: #t:limb_t -> k:BE.exp t -> bn_mod_exp_safe_st t k.BE.mont.BM.bn.BN.len
+let bn_mod_exp_ct_safe #t k n a bBits b res =
   [@inline_let] let len = k.BE.mont.BM.bn.BN.len in
   let h0 = ST.get () in
   let is_valid_m = k.BE.exp_check n a bBits b in
   let nBits = size (bits t) *! BB.unsafe_size_from_limb (BL.bn_get_top_index len n) in
 
-  BE.bn_mod_exp_mont_ladder k.BE.mont k.BE.ct_mod_exp_precomp nBits n a bBits b res;
+  BE.bn_mod_exp_ct k.BE.mont k.BE.ct_mod_exp_precomp nBits n a bBits b res;
   let h1 = ST.get () in
   mapT len res (logand is_valid_m) res;
   SD.bn_mask_lemma (as_seq h1 res) is_valid_m;
 
   if BB.unsafe_bool_of_limb is_valid_m then begin
     SL.bn_low_bound_bits_lemma #t #(v len) (as_seq h0 n);
-    SE.bn_mod_exp_mont_ladder_lemma (v len) (v nBits) (as_seq h0 n) (as_seq h0 a) (v bBits) (as_seq h0 b);
+    SE.bn_mod_exp_ct_lemma (v len) (v nBits) (as_seq h0 n) (as_seq h0 a) (v bBits) (as_seq h0 b);
     assert (SE.bn_mod_exp_post (as_seq h0 n) (as_seq h0 a) (v bBits) (as_seq h0 b) (as_seq h1 res)) end;
   BB.unsafe_bool_of_limb is_valid_m
 
@@ -231,14 +231,14 @@ let bn_mod_inv_prime_safe_st (t:limb_t) (len:BN.meta_len t) =
 
 
 inline_for_extraction noextract
-val bn_mod_inv_prime_safe: #t:limb_t -> k:BE.exp t -> bn_mod_inv_prime_safe_st t k.BE.mont.BM.bn.BN.len
-let bn_mod_inv_prime_safe #t k n a res =
+val bn_mod_inv_prime_raw_safe: #t:limb_t -> k:BE.exp t -> bn_mod_inv_prime_safe_st t k.BE.mont.BM.bn.BN.len
+let bn_mod_inv_prime_raw_safe #t k n a res =
   [@inline_let] let len = k.BE.mont.BM.bn.BN.len in
   let h0 = ST.get () in
   let is_valid_m = BI.bn_check_bn_mod_inv_prime #t k n a in
   let nBits = size (bits t) *! BB.unsafe_size_from_limb (BL.bn_get_top_index len n) in
 
-  BI.bn_mod_inv_prime k nBits n a res;
+  BI.bn_mod_inv_prime_raw k nBits n a res;
   let h1 = ST.get () in
   mapT len res (logand is_valid_m) res;
   SD.bn_mask_lemma (as_seq h1 res) is_valid_m;
