code/bignum/Hacl.Spec.Bignum.Exponentiation.fst
@@ -6,6 +6,7 @@ open Lib.IntTypes
 open Lib.Sequence
 
 open Hacl.Spec.Bignum.Definitions
+
 include Hacl.Spec.Bignum.ExpBM
 include Hacl.Spec.Bignum.ExpFW
 
@@ -13,26 +14,26 @@ module BM = Hacl.Spec.Bignum.Montgomery
 
 #reset-options "--z3rlimit 50 --fuel 0 --ifuel 0"
 
-let bn_mod_exp #t nLen nBits n a bBits b =
+let bn_mod_exp_raw #t nLen nBits n a bBits b =
   let r2 = BM.bn_precomp_r2_mod_n nBits n in
-  bn_mod_exp_precompr2 nLen n a bBits b r2
+  bn_mod_exp_raw_precompr2 nLen n a bBits b r2
 
 
-let bn_mod_exp_lemma #t nLen nBits n a bBits b =
-  let r2 = BM.bn_precomp_r2_mod_n nBits n in
-  BM.bn_precomp_r2_mod_n_lemma nBits n;
-  bn_mod_exp_precompr2_lemma nLen n a bBits b r2
-
-
-let bn_mod_exp_mont_ladder #t nLen nBits n a bBits b =
-  let r2 = BM.bn_precomp_r2_mod_n nBits n in
-  bn_mod_exp_mont_ladder_precompr2 nLen n a bBits b r2
-
-
-let bn_mod_exp_mont_ladder_lemma #t nLen nBits n a bBits b =
+let bn_mod_exp_raw_lemma #t nLen nBits n a bBits b =
   let r2 = BM.bn_precomp_r2_mod_n nBits n in
   BM.bn_precomp_r2_mod_n_lemma nBits n;
-  bn_mod_exp_mont_ladder_precompr2_lemma nLen n a bBits b r2
+  bn_mod_exp_raw_precompr2_lemma nLen n a bBits b r2
+
+
+let bn_mod_exp_ct #t nLen nBits n a bBits b =
+  let r2 = BM.bn_precomp_r2_mod_n nBits n in
+  bn_mod_exp_ct_precompr2 nLen n a bBits b r2
+
+
+let bn_mod_exp_ct_lemma #t nLen nBits n a bBits b =
+  let r2 = BM.bn_precomp_r2_mod_n nBits n in
+  BM.bn_precomp_r2_mod_n_lemma nBits n;
+  bn_mod_exp_ct_precompr2_lemma nLen n a bBits b r2
 
 
 let bn_mod_exp_fw #t nLen nBits n a bBits b l =
